perf: speed up bv_decide reflection using Lean.RArray (#6288)
This PR uses Lean.RArray in bv_decide's reflection proofs. Giving
speedups on problems with lots of variables.

Implement like #6068, speedup:
```
# before
λ hyperfine "lean +nightly-2024-12-02 tests/lean/run/bv_reflection_stress.lean"
Benchmark 1: lean +nightly-2024-12-02 tests/lean/run/bv_reflection_stress.lean
  Time (mean ± σ):      1.939 s ±  0.007 s    [User: 1.549 s, System: 0.104 s]
  Range (min … max):    1.928 s …  1.947 s    10 runs
# after
λ hyperfine "lean tests/lean/run/bv_reflection_stress.lean"                                                                                                                                                                                                                        
Benchmark 1: lean tests/lean/run/bv_reflection_stress.lean
  Time (mean ± σ):      1.409 s ±  0.006 s    [User: 1.058 s, System: 0.073 s]
  Range (min … max):    1.401 s …  1.419 s    10 runs
```

src/Std/Tactic/BVDecide/Bitblast/BVExpr/Basic.lean
@@ -6,6 +6,7 @@ Authors: Henrik Böving
 prelude
 import Init.Data.Hashable
 import Init.Data.BitVec
+import Init.Data.RArray
 import Std.Tactic.BVDecide.Bitblast.BoolExpr.Basic
 
 /-!
@@ -279,20 +280,20 @@ structure PackedBitVec where
 /--
 The notion of variable assignments for `BVExpr`.
 -/
-abbrev Assignment := List PackedBitVec
+abbrev Assignment := Lean.RArray PackedBitVec
 
 /--
 Get the value of a `BVExpr.var` from an `Assignment`.
 -/
-def Assignment.getD (assign : Assignment) (idx : Nat) : PackedBitVec :=
-  List.getD assign idx ⟨BitVec.zero 0⟩
+def Assignment.get (assign : Assignment) (idx : Nat) : PackedBitVec :=
+  Lean.RArray.get assign idx
 
 /--
 The semantics for `BVExpr`.
 -/
 def eval (assign : Assignment) : BVExpr w → BitVec w
   | .var idx =>
-    let ⟨bv⟩ := assign.getD idx
+    let ⟨bv⟩ := assign.get idx
     bv.truncate w
   | .const val => val
   | .zeroExtend v expr => BitVec.zeroExtend v (eval assign expr)
@@ -307,7 +308,7 @@ def eval (assign : Assignment) : BVExpr w → BitVec w
   | .arithShiftRight lhs rhs => BitVec.sshiftRight' (eval assign lhs) (eval assign rhs)
 
 @[simp]
-theorem eval_var : eval assign ((.var idx) : BVExpr w) = (assign.getD idx).bv.truncate _ := by
+theorem eval_var : eval assign ((.var idx) : BVExpr w) = (assign.get idx).bv.truncate _ := by
   rfl
 
 @[simp]
